iris/BioInv.v
@@ -719,6 +719,9 @@ Section BioInv.
      (keys AND mass: only the stamp is existential, R-1) *)
   Definition bstok (bn : bio_names) (k : nat) (pidv dev bno : mword 32) : iProp Σ :=
     (sleeplocked (snd (bn_slk bn k)) (buf_lock (bnode k)) pidv ∗
+     (* the sleeplock's exclusivity token rides the handle: the box no
+        longer takes it (endgame plan §6⁶(A)) *)
+     bown bn k ∗
      bref_tok0 bn k ∗
      ∃ t : nat, CtxBox.l2_hold (X := bio_x) (bn_box bn k) (dev, bno) {[((dev, bno), t) := 1%Qp]})%I.
 
@@ -1026,7 +1029,7 @@ Section BioBox.
 
   (* THE BOX *)
   Definition buf_box (bn : bio_names) (V : bio_view Σ) (k : nat) : iProp Σ :=
-    is_box (bhdr bn V k) (brest k) emp (bown bn k) bioxN (bn_box bn k).
+    is_box (bhdr bn V k) (brest k) emp (bioxN .@ k) (bn_box bn k).
   Global Instance buf_box_persistent bn V k : Persistent (buf_box bn V k).
   Proof. rewrite /buf_box /is_box. apply _. Qed.
 
@@ -1054,17 +1057,19 @@ Section BioBox.
       bhdr bn V k (sr_ident r) x0 ξ.
   Proof.
     iIntros (HE Hw HKd) "#Hbox Hrun #Hfl Hrd Hc".
+    assert (HEk : ↑(bioxN .@ k) ⊆ E) by (etrans; [apply nclose_subseteq | exact HE]).
     iMod (own_unit (authUR (gmapUR (bio_id * nat) ufracR)) (bx_stamps (bn_box bn k))) as "Hf0".
     assert (Hq0 : qsum (∅ : gmap (bio_id * nat) ufrac) = nat_Qc 0).
     { rewrite /qsum map_fold_empty /nat_Qc /=. symmetry. apply Z2Qc_inj_0. }
     assert (Hm0 : (max_stamp (∅ : gmap (bio_id * nat) ufrac) <= 0)%nat).
     { rewrite /max_stamp map_fold_empty. lia. }
-    iMod (CtxBox.box_withdraw_L1 (bhdr bn V k) (brest k) emp%I (bown bn k)
-            bioxN (bn_box bn k) ξ r 0 ∅ Kd 0 E HE Hw Hq0 HKd Hm0
-            with "Hbox Hrun Hfl [] [] Hrd Hc [Hf0]") as "(Hrun & Hc & Hout)".
+    iMod (CtxBox.box_withdraw_L1 (bhdr bn V k) (brest k) emp%I
+            (bioxN .@ k) (bn_box bn k) ξ r 0 ∅ Kd 0 E HEk Hw Hq0 HKd Hm0
+            with "Hbox Hrun Hfl [] [] Hrd Hc [Hf0] []") as "(Hrun & Hc & Hout)".
     { iApply TsoCtx.ctx_floor_0. }
     { rewrite /max_stamp map_fold_empty. iApply TsoGhost.llb_0. }
     { rewrite /stamps_frag. iExact "Hf0". }
+    { done. }
     iDestruct "Hout" as (x0 T0) "(%HT0 & Hrd & Hhdr)".
     iModIntro. iFrame "Hrun Hc". iExists x0, T0. iFrame "Hrd Hhdr". iPureIntro. lia.
   Qed.
@@ -1085,10 +1090,11 @@ Section BioBox.
                 bref_ghost bn k dev bno ∗ llb loglen_name T'.
   Proof.
     iIntros (HE) "#Hbox Hrun Hrd Hc Hhdr".
-    iMod (CtxBox.box_deposit_L1 (bhdr bn V k) (brest k) emp%I (bown bn k)
-            bioxN (bn_box bn k) ξ
-            (SlotReg Td true i0 (Some (x0, T0))) 0 (dev, bno) x0 T0 E HE eq_refl eq_refl
-            with "Hbox Hrun Hrd Hc Hhdr") as "(Hrun & %T' & Hrd & Hc & Href & #Hllb)".
+    assert (HEk : ↑(bioxN .@ k) ⊆ E) by (etrans; [apply nclose_subseteq | exact HE]).
+    iMod (CtxBox.box_deposit_L1 (bhdr bn V k) (brest k) emp%I
+            (bioxN .@ k) (bn_box bn k) ξ
+            (SlotReg Td true i0 (Some (x0, T0))) 0 (dev, bno) x0 T0 E HEk eq_refl eq_refl
+            with "Hbox Hrun Hrd Hc Hhdr") as "(Hrun & _ & %T' & Hrd & Hc & Href & #Hllb)".
     iModIntro. iFrame "Hrun". iExists T'. iFrame "Hrd Hllb".
     iSplitL "Hc"; [iExact "Hc"|].
     rewrite /bref_ghost. iExists T'.
@@ -1107,8 +1113,9 @@ Section BioBox.
     reg_drop bn k r ∗ reg_cnt bn k (S c) ∗ bref_ghost bn k dev bno.
   Proof.
     iIntros (HE Hw Hid) "#Hbox Hrd Hc".
-    iMod (CtxBox.box_ref_incr (bhdr bn V k) (brest k) emp%I (bown bn k)
-            bioxN (bn_box bn k) r c E HE Hw
+    assert (HEk : ↑(bioxN .@ k) ⊆ E) by (etrans; [apply nclose_subseteq | exact HE]).
+    iMod (CtxBox.box_ref_incr (bhdr bn V k) (brest k) emp%I
+            (bioxN .@ k) (bn_box bn k) r c E HEk Hw
             with "Hbox Hrd Hc") as "(Hrd & Hc & %T & Href)".
     iModIntro. iFrame "Hrd Hc". rewrite /bref_ghost. iExists T. rewrite Hid. iExact "Href".
   Qed.
@@ -1129,11 +1136,12 @@ Section BioBox.
       llb loglen_name td'.
   Proof.
     iIntros (HE Hw) "#Hbox Hrd #Hllb Hc Href". iDestruct "Href" as (t) "Href".
+    assert (HEk : ↑(bioxN .@ k) ⊆ E) by (etrans; [apply nclose_subseteq | exact HE]).
     assert (Hq1 : qsum ({[((dev, bno), t) := 1%Qp]} : gmap (bio_id * nat) ufrac) = nat_Qc 1).
     { rewrite /qsum map_fold_singleton /qsum_step Qcplus_0_r Qp_to_Qc_1 /nat_Qc /=. symmetry. apply Z2Qc_inj_1. }
-    iMod (CtxBox.box_ref_decr (bhdr bn V k) (brest k) emp%I (bown bn k)
-            bioxN (bn_box bn k) r c (dev, bno)
-            {[((dev, bno), t) := 1%Qp]} E HE Hw Hq1
+    iMod (CtxBox.box_ref_decr (bhdr bn V k) (brest k) emp%I
+            (bioxN .@ k) (bn_box bn k) r c (dev, bno)
+            {[((dev, bno), t) := 1%Qp]} E HEk Hw Hq1
             with "Hbox Hrd Hllb Hc Href") as "(Hrd & Hc & #Hllb')".
     iModIntro. iExists (Nat.max (sr_td r) (max_stamp {[((dev, bno), t) := 1%Qp]})).
     iSplitR; [iPureIntro; lia|]. iFrame "Hrd Hc Hllb'".
@@ -1153,18 +1161,18 @@ Section BioBox.
     TsoCtx.ctx_floor ξ Kt -∗
     TsoCtx.ctx_floor ξ Kp -∗
     CtxBox.reference (X := bio_x) (bn_box bn k) (dev, bno) {[((dev, bno), t) := 1%Qp]} -∗
-    bown bn k -∗
     reg_park bn k s0 ={E}=∗
     TsoCtx.own_context ξ ∗ buf_bundle_at bn V k ξ dev bno ∗
     CtxBox.l2_hold (X := bio_x) (bn_box bn k) (dev, bno) {[((dev, bno), t) := 1%Qp]}.
   Proof.
-    iIntros (HE Hs0 HKt HKp) "#Hbox Hrun #Hflt #Hflp Href Htok Hrp".
+    iIntros (HE Hs0 HKt HKp) "#Hbox Hrun #Hflt #Hflp Href Hrp".
+    assert (HEk : ↑(bioxN .@ k) ⊆ E) by (etrans; [apply nclose_subseteq | exact HE]).
     assert (Hmt : (max_stamp ({[((dev, bno), t) := 1%Qp]} : gmap (bio_id * nat) ufrac) <= Kt)%nat).
     { rewrite /max_stamp map_fold_singleton /max_step /=. lia. }
-    iMod (CtxBox.box_checkout (bhdr bn V k) (brest k) emp%I (bown bn k)
-            (bown_excl bn k) bioxN (bn_box bn k) ξ (dev, bno)
-            {[((dev, bno), t) := 1%Qp]} s0 Kt Kp E HE Hs0 Hmt HKp
-            with "Hbox Hrun Hflt Hflp Href [] Htok Hrp") as "(Hrun & Hbun & Hhold)".
+    iMod (CtxBox.box_checkout (bhdr bn V k) (brest k) emp%I
+            (bioxN .@ k) (bn_box bn k) ξ (dev, bno)
+            {[((dev, bno), t) := 1%Qp]} s0 Kt Kp E HEk Hs0 Hmt HKp
+            with "Hbox Hrun Hflt Hflp Href [] Hrp") as "(Hrun & Hbun & Hhold)".
     { done. }
     iModIntro. iFrame "Hrun Hhold". iExact "Hbun".
   Qed.
@@ -1178,17 +1186,18 @@ Section BioBox.
     TsoCtx.own_context ξ -∗
     buf_bundle_at bn V k ξ dev bno -∗
     CtxBox.l2_hold (X := bio_x) (bn_box bn k) (dev, bno) {[((dev, bno), t) := 1%Qp]} ={E}=∗
-    TsoCtx.own_context ξ ∗ bown bn k ∗
+    TsoCtx.own_context ξ ∗
     ∃ T' : nat, reg_park bn k (L2Reg T' None) ∗ bref_ghost bn k dev bno ∗ llb loglen_name T'.
   Proof.
     iIntros (HE) "#Hbox Hrun Hbun Hhold".
-    iMod (CtxBox.box_park (bhdr bn V k) (brest k) emp%I (bown bn k)
-            (bhdr_excl bn V k) (brest_excl k) bioxN (bn_box bn k) ξ (dev, bno)
-            {[((dev, bno), t) := 1%Qp]} E HE
-            with "Hbox Hrun Hbun Hhold") as "(Hrun & _ & Htok & %T' & %q & %Hq & Hrp & Href & #Hllb)".
+    assert (HEk : ↑(bioxN .@ k) ⊆ E) by (etrans; [apply nclose_subseteq | exact HE]).
+    iMod (CtxBox.box_park (bhdr bn V k) (brest k) emp%I
+            (bioxN .@ k) (bn_box bn k) ξ (dev, bno)
+            {[((dev, bno), t) := 1%Qp]} E HEk
+            with "Hbox Hrun Hbun Hhold") as "(Hrun & _ & %T' & %q & %Hq & Hrp & Href & #Hllb)".
     assert (q = 1%Qp) as ->.
     { apply Qp.to_Qc_inj_iff. rewrite Hq /qsum map_fold_singleton /qsum_step. by rewrite Qcplus_0_r. }
-    iModIntro. iFrame "Hrun Htok". iExists T'. iFrame "Hrp Hllb".
+    iModIntro. iFrame "Hrun". iExists T'. iFrame "Hrp Hllb".
     rewrite /bref_ghost. iExists T'. iExact "Href".
   Qed.
 
@@ -1566,8 +1575,8 @@ Section BioBox.
       iExists bs. iSplitL "Hv Hdev Hbno Hpay".
       { iExists false. cbn [fst snd]. cbv iota. iFrame "Hv Hdev Hbno Hpay". }
       iFrame "Hdk Hdata". done. }
-    iMod (CtxBox.box_alloc_at (bhdr bn V k) (brest k) emp%I (bown bn k)
-            bioxN (bn_box bn k) cur_ctx
+    iMod (CtxBox.box_alloc_at_halves (bhdr bn V k) (brest k) emp%I
+            (bioxN .@ k) (bn_box bn k) cur_ctx
             (mword_of_int 0 : mword 32, mword_of_int 0 : mword 32) E
             with "Hrun Hst Hc [Hrd] Hrp Hbun") as "(Hrun & %Tb & #Hbx & Hrd & #Hllb)".
     { rewrite /bn_box /=. iExact "Hrd". }
